$$
    \left( 
        2 \cdot 4^{x^2-3x}
    \right)^2
    =
    2^{x-1}
$$
Wurzel ziehen
$$
    2 \cdot 4^{x^2-3x}
    =
    2^{\frac{x-1}{2}}
$$
Beide Seiten durch 2
$$
    4^{x^2-3x}
    =
    2^{\frac{x-3}{2}}
$$
Links aus der 4 eine $2^2$
$$
    2^{2x^2-6x}
    =
    2^{\frac{x-3}{2}}
$$
Nur die Exponenten betrachten
$$
\begin{aligned}
    2x^2-6x
    &=
    \frac{x-3}{2}
\\    
    x^2-\frac{13}{4}x + \frac{3}{4}
    &=
    0
\\    
    x_{1,2} &= \frac{13}{8} \pm \sqrt{\frac{169}{64} - \frac{48}{64}}
\end{aligned}
$$

Daraus ergibt sich $x_1+x_2 = 2\cdot\frac{13}{8} = \frac{13}{4} = 3.25$.